Prove hom_span

Generators.thy
@@ -19,56 +19,51 @@ text {* The span of a set of subgroup generators, i.e. the generated subgroup, c
 be defined inductively or as the intersection of all subgroups containing the
 generators. Here, we define it inductively and proof the equivalence *}
 
-inductive_set (in group) gen_span :: "'a set \<Rightarrow> 'a set" ("\<guillemotleft>_\<guillemotright>" 81)
-  for gens :: "'a set"
-where gen_one [intro!, simp]: "\<one> \<in> \<guillemotleft>gens\<guillemotright>"
-    | gen_gens: "x \<in> gens \<Longrightarrow> x \<in> \<guillemotleft>gens\<guillemotright>"
-    | gen_inv: "x \<in> \<guillemotleft>gens\<guillemotright> \<Longrightarrow> inv x \<in> \<guillemotleft>gens\<guillemotright>"
-    | gen_mult: "\<lbrakk> x \<in> \<guillemotleft>gens\<guillemotright>; y \<in> \<guillemotleft>gens\<guillemotright> \<rbrakk> \<Longrightarrow>  x \<otimes> y \<in> \<guillemotleft>gens\<guillemotright>"
-
-(*
-definition (in group) gen_subgroup :: "'a set \<Rightarrow> ('a,'b) monoid_scheme" ("\<guillemotleft>_\<guillemotright>" 80)
- where "\<guillemotleft>gens\<guillemotright> = G (|carrier := \<guillemotleft>gens\<guillemotright> |)"
-*)
+inductive_set gen_span :: "('a,'b) monoid_scheme \<Rightarrow> 'a set \<Rightarrow> 'a set" ("\<guillemotleft>_\<guillemotright>\<index>")
+  for G and gens
+where gen_one [intro!, simp]: "\<one>\<^bsub>G\<^esub> \<in> \<guillemotleft>gens\<guillemotright>\<^bsub>G\<^esub>"
+    | gen_gens: "x \<in> gens \<Longrightarrow> x \<in> \<guillemotleft>gens\<guillemotright>\<^bsub>G\<^esub>"
+    | gen_inv: "x \<in> \<guillemotleft>gens\<guillemotright>\<^bsub>G\<^esub> \<Longrightarrow> inv\<^bsub>G\<^esub> x \<in> \<guillemotleft>gens\<guillemotright>\<^bsub>G\<^esub>"
+    | gen_mult: "\<lbrakk> x \<in> \<guillemotleft>gens\<guillemotright>\<^bsub>G\<^esub>; y \<in> \<guillemotleft>gens\<guillemotright>\<^bsub>G\<^esub> \<rbrakk> \<Longrightarrow>  x \<otimes>\<^bsub>G\<^esub> y \<in> \<guillemotleft>gens\<guillemotright>\<^bsub>G\<^esub>"
 
 lemma (in group) gen_span_closed:
   assumes "gens \<subseteq> carrier G"
-  shows "\<guillemotleft>gens\<guillemotright> \<subseteq> carrier G"
+  shows "\<guillemotleft>gens\<guillemotright>\<^bsub>G\<^esub> \<subseteq> carrier G"
 proof (* How can I do this in one "by" line? *)
   fix x
-  from assms show "x \<in> \<guillemotleft>gens\<guillemotright> \<Longrightarrow> x \<in> carrier G"
+  from assms show "x \<in> \<guillemotleft>gens\<guillemotright>\<^bsub>G\<^esub> \<Longrightarrow> x \<in> carrier G"
     by -(induct rule:gen_span.induct, auto)
 qed
 
 lemma (in group) gen_subgroup_is_subgroup: 
-      "gens \<subseteq> carrier G \<Longrightarrow> \<guillemotleft>gens\<guillemotright> \<le> G"
+      "gens \<subseteq> carrier G \<Longrightarrow> \<guillemotleft>gens\<guillemotright>\<^bsub>G\<^esub> \<le> G"
 by(rule subgroupI)(auto intro:gen_span.intros simp add:gen_span_closed)
 
 lemma (in group) gen_subgroup_is_smallest_containing:
   assumes "gens \<subseteq> carrier G"
-    shows "\<Inter>{H. H \<le> G \<and> gens \<subseteq> H} = \<guillemotleft>gens\<guillemotright>"
+    shows "\<Inter>{H. H \<le> G \<and> gens \<subseteq> H} = \<guillemotleft>gens\<guillemotright>\<^bsub>G\<^esub>"
 proof
-  show "\<guillemotleft>gens\<guillemotright> \<subseteq> \<Inter>{H. H \<le> G \<and> gens \<subseteq> H}"
+  show "\<guillemotleft>gens\<guillemotright>\<^bsub>G\<^esub> \<subseteq> \<Inter>{H. H \<le> G \<and> gens \<subseteq> H}"
   proof(rule Inf_greatest)
     fix H
     assume "H \<in> {H. H \<le> G \<and> gens \<subseteq> H}"
     hence "H \<le> G" and "gens \<subseteq> H" by auto
-    show "\<guillemotleft>gens\<guillemotright> \<subseteq> H"
+    show "\<guillemotleft>gens\<guillemotright>\<^bsub>G\<^esub> \<subseteq> H"
     proof
       fix x
       from `H \<le> G` and `gens \<subseteq> H`
-      show "x \<in> \<guillemotleft>gens\<guillemotright> \<Longrightarrow> x \<in> H"
+      show "x \<in> \<guillemotleft>gens\<guillemotright>\<^bsub>G\<^esub> \<Longrightarrow> x \<in> H"
        unfolding subgroup_def
        by -(induct rule:gen_span.induct, auto)
     qed
   qed
 next
   from `gens \<subseteq> carrier G`
-  have "\<guillemotleft>gens\<guillemotright> \<le> G" by (rule gen_subgroup_is_subgroup)
+  have "\<guillemotleft>gens\<guillemotright>\<^bsub>G\<^esub> \<le> G" by (rule gen_subgroup_is_subgroup)
   moreover
-  have "gens \<subseteq> \<guillemotleft>gens\<guillemotright>" by (auto intro:gen_span.intros)
+  have "gens \<subseteq> \<guillemotleft>gens\<guillemotright>\<^bsub>G\<^esub>" by (auto intro:gen_span.intros)
   ultimately
-  show "\<Inter>{H. H \<le> G \<and> gens \<subseteq> H} \<subseteq> \<guillemotleft>gens\<guillemotright>"
+  show "\<Inter>{H. H \<le> G \<and> gens \<subseteq> H} \<subseteq> \<guillemotleft>gens\<guillemotright>\<^bsub>G\<^esub>"
     by(auto intro:Inter_lower)
 qed
 
@@ -83,7 +78,7 @@ lemma hom_unique_on_span:
       and "h \<in> hom G H"
       and "h' \<in> hom G H"
       and "\<forall>g \<in> gens. h g = h' g"
-  shows "\<forall>x \<in> group.gen_span G gens. h x = h' x"
+  shows "\<forall>x \<in> \<guillemotleft>gens\<guillemotright>\<^bsub>G\<^esub>. h x = h' x"
 proof
   interpret G: group G by fact
   interpret H: group H by fact
@@ -91,9 +86,9 @@ proof
   interpret h': group_hom G H h' by unfold_locales fact
 
   fix x
-  from `gens \<subseteq> carrier G` have "\<guillemotleft>gens\<guillemotright> \<subseteq> carrier G" by (rule G.gen_span_closed)
-  with assms show "x \<in> \<guillemotleft>gens\<guillemotright> \<Longrightarrow> h x = h' x" apply -
-  proof(induct rule:G.gen_span.induct)
+  from `gens \<subseteq> carrier G` have "\<guillemotleft>gens\<guillemotright>\<^bsub>G\<^esub> \<subseteq> carrier G" by (rule G.gen_span_closed)
+  with assms show "x \<in> \<guillemotleft>gens\<guillemotright>\<^bsub>G\<^esub> \<Longrightarrow> h x = h' x" apply -
+  proof(induct rule:gen_span.induct)
     case (gen_mult x y)
       hence x: "x \<in> carrier G" and y: "y \<in> carrier G" and
             hx: "h x = h' x" and hy: "h y = h' y" by auto
@@ -109,10 +104,9 @@ text {* There is no definition for @{text gens} is a generating set of
 text {* The following is application of @{text hom_unique_on_span} on a generating
   set of the whole group. *}
 
-
 lemma (in group) hom_unique_by_gens:
   assumes "group H"
-      and gens: "\<guillemotleft>gens\<guillemotright> = carrier G"
+      and gens: "\<guillemotleft>gens\<guillemotright>\<^bsub>G\<^esub> = carrier G"
       and "h \<in> hom G H"
       and "h' \<in> hom G H"
       and "\<forall>g \<in> gens. h g = h' g"
@@ -121,10 +115,65 @@ proof
   fix x
 
   from gens have "gens \<subseteq> carrier G" by (auto intro:gen_span.gen_gens)
-  with assms and group_axioms have r: "\<forall>x \<in> group.gen_span G gens. h x = h' x"
+  with assms and group_axioms have r: "\<forall>x \<in> \<guillemotleft>gens\<guillemotright>\<^bsub>G\<^esub>. h x = h' x"
     by -(erule hom_unique_on_span, auto)
   with gens show "x \<in> carrier G \<Longrightarrow> h x = h' x" by auto
 qed
+
+lemma (in group_hom) hom_span:
+  assumes "gens \<subseteq> carrier G"
+  shows "h ` (\<guillemotleft>gens\<guillemotright>\<^bsub>G\<^esub>) = \<guillemotleft>h ` gens\<guillemotright>\<^bsub>H\<^esub>"
+proof(rule set_ext, rule iffI)
+  from `gens \<subseteq> carrier G`
+  have "\<guillemotleft>gens\<guillemotright>\<^bsub>G\<^esub> \<subseteq> carrier G" by (rule G.gen_span_closed)
+
+  fix y
+  assume "y \<in> h ` \<guillemotleft>gens\<guillemotright>\<^bsub>G\<^esub>"
+  then obtain x where "x \<in> \<guillemotleft>gens\<guillemotright>\<^bsub>G\<^esub>" and "y = h x" by auto
+  from `x \<in> \<guillemotleft>gens\<guillemotright>\<^bsub>G\<^esub>`
+  have "h x \<in> \<guillemotleft>h ` gens\<guillemotright>\<^bsub>H\<^esub>"
+  proof(induct x)
+    print_cases
+    case (gen_inv x)
+    hence "x \<in> carrier G" and "h x \<in> \<guillemotleft>h ` gens\<guillemotright>\<^bsub>H\<^esub>"
+      using `\<guillemotleft>gens\<guillemotright>\<^bsub>G\<^esub> \<subseteq> carrier G`
+      by auto
+    thus ?case by (auto intro:gen_span.intros)
+  next
+    case (gen_mult x y)
+    hence "x \<in> carrier G" and "h x \<in> \<guillemotleft>h ` gens\<guillemotright>\<^bsub>H\<^esub>"
+    and   "y \<in> carrier G" and "h y \<in> \<guillemotleft>h ` gens\<guillemotright>\<^bsub>H\<^esub>"
+      using `\<guillemotleft>gens\<guillemotright>\<^bsub>G\<^esub> \<subseteq> carrier G`
+      by auto
+    thus ?case by (auto intro:gen_span.intros)
+  qed(auto intro: gen_span.intros)
+  with `y = h x`
+  show "y \<in> \<guillemotleft>h ` gens\<guillemotright>\<^bsub>H\<^esub>" by simp
+next
+  fix x
+  show "x \<in> \<guillemotleft>h ` gens\<guillemotright>\<^bsub>H\<^esub> \<Longrightarrow> x \<in> h ` \<guillemotleft>gens\<guillemotright>"
+  proof(induct x rule:gen_span.induct)
+  print_cases
+    case (gen_inv y)
+      then  obtain x where "y = h x" and "x \<in> \<guillemotleft>gens\<guillemotright>" by auto
+      moreover
+      hence "x \<in> carrier G"  using `gens \<subseteq> carrier G` 
+        by (auto dest:G.gen_span_closed)
+      ultimately show ?case 
+        by (auto intro:hom_inv[THEN sym] rev_image_eqI gen_span.gen_inv simp del:group_hom.hom_inv hom_inv)
+  next
+   case (gen_mult y y')
+      then  obtain x and x'
+        where "y = h x" and "x \<in> \<guillemotleft>gens\<guillemotright>"
+        and "y' = h x'" and "x' \<in> \<guillemotleft>gens\<guillemotright>" by auto
+      moreover
+      hence "x \<in> carrier G" and "x' \<in> carrier G" using `gens \<subseteq> carrier G` 
+        by (auto dest:G.gen_span_closed)
+      ultimately show ?case
+        by (auto intro:hom_mult[THEN sym] rev_image_eqI gen_span.gen_mult simp del:group_hom.hom_mult hom_mult)
+  qed(auto intro:rev_image_eqI intro:gen_span.intros)
+qed
+
 
 subsection {* Product of a list of group elements *}
 
@@ -151,3 +200,4 @@ by(induct xs rule:rev_induct)(auto simp add: m_assoc)
 
 
 end
+
